more tests and format

code/c/test.c
@@ -1,0 +1,32 @@
+#include "adler32.h"
+#include <stdint.h>
+#include <stdio.h>
+#include <string.h>
+#include <assert.h>
+
+const char *GREEN = "\033[32m";
+const char *RESET = "\033[0m";
+
+int32_t main(void)
+{
+    char *input1 = "Wikipedia";
+    assert(adler32(input1, strlen(input1)) == 300286872);
+
+    char *input2 = "Algorithms";
+    assert(adler32(input2, strlen(input2)) == 363791387);
+
+    char *input3 = "Hello, World!";
+    assert(adler32(input3, strlen(input3)) == 530449514);
+
+    char input4[] = {4, 1, 6, 3, 10};
+    assert(adler32(input4, 5) == 4128793);
+
+    char input5[] = {};
+    assert(adler32(input5, 0) == 1);
+
+    char input6[] = {1};
+    assert(adler32(input6, 1) == 131074);
+
+    printf("%sAll tests passed!\n%s", GREEN, RESET);
+    return 0;
+}
