code/Impl.Adler32.fst
@@ -1,32 +1,60 @@
 module Impl.Adler32
 
-module U8 = FStar.UInt8
-module U32 = FStar.UInt32
-module N = FStar.Pervasives.Native
-module P = LowStar.Printf
-module U32 = FStar.UInt32
+open FStar.Mul
 
 open FStar.HyperStack.ST
-open LowStar.BufferOps
-open LowStar.Buffer
 
-let square1 (x: U32.t): Stack U32.t (fun _ -> True) (fun _ _ _ -> True) =
-  FStar.UInt32.( x *%^ x )
+module B = LowStar.Buffer
 
-let square2 (x: U32.t): Stack U32.t (fun _ -> True) (fun _ _ _ -> True) =
+module C = LowStar.ConstBuffer
+
+module S = FStar.Seq
+
+module HS = FStar.HyperStack
+
+module U8 = FStar.UInt8
+
+module U32 = FStar.UInt32
+
+module SPEC = Spec.Adler32
+
+noextract inline_for_extraction
+let cast (d: U8.t) : U32.t = FStar.Int.Cast.uint8_to_uint32 d
+
+#push-options "--query_stats --max_fuel 5000 --max_ifuel 5000 --z3rlimit 600"
+
+val adler32 (data: C.const_buffer U8.t) (len: U32.t) : Stack U32.t
+  (requires fun (h0: HS.mem) -> C.live h0 data /\ C.length data = U32.v len)
+  (ensures fun (h0: HS.mem) (x: U32.t) (h1: HS.mem) ->
+    C.live h0 data /\ C.live h1 data /\
+    (*U32.v x == Spec.Adler32.adler32(C.as_seq h0 data) /\*)
+    True)
+
+let adler32 data len =
+  let open LowStar.BufferOps in
+  let open U32 in
   push_frame ();
-  let b = alloca 0ul 1ul in
+  let a:B.buffer U32.t = B.alloca 1ul 1ul in
+  let b:B.buffer U32.t = B.alloca 0ul 1ul in
+  let inv (h: HS.mem) (i: nat) : Type0 =
+    let a_nat = U32.v (B.get h a 0) in
+    let b_nat = U32.v (B.get h b 0) in
+    i <= U32.v len /\ B.live h a /\ B.live h b /\ C.live h data /\ a_nat < 65521 /\ b_nat < 65521 /\
+    // a_nat == Spec.Adler32.sum_plus_one (S.slice (C.as_seq h data) 0 i) % 65521 /\
+    // b_nat == Spec.Adler32.weighted_sum_plus_len (S.slice (C.as_seq h data) 0 i) % 65521 /\
+    // b_nat * (pow2 16 ) + a_nat == Spec.Adler32.adler32 (S.slice (C.as_seq h data) 0 i) /\
+    True
+  in
+  let body (i: U32.t{U32.v 0ul <= U32.v i /\ U32.v i < U32.v len})
+      : Stack unit
+        (requires fun h -> inv h (U32.v i))
+        (ensures fun h0 _ h1 -> (inv h0 (U32.v i) /\ inv h1 ((U32.v i) + 1))) =
+    a.(0ul) <- (a.(0ul) +^ cast (C.index data i)) %^ 65521ul;
+    b.(0ul) <- (b.(0ul) +^ a.(0ul)) %^ 65521ul
+  in
+  C.Loops.for 0ul len inv body;
+  let return:U32.t = U32.logor (U32.shift_left b.(0ul) 16ul) a.(0ul) in
   pop_frame ();
-  FStar.UInt32.( x *%^ x )
+  return
 
-let adler32 (data: buffer U8.t) (len: U32.t) : U32.t =
-  let a = 1ul in
-  let b = 0ul in
-
-  a 
-
-let main (): St Int32.t =
-  push_frame ();
-  P.(printf "Hello, World!\n" done);
-  pop_frame ();
-  0l
+#pop-options
