code/Spec.Adler32.fst
@@ -1,0 +1,72 @@
+module Spec.Adler32
+
+open FStar.Mul
+
+open FStar.HyperStack.ST
+
+module C = LowStar.ConstBuffer
+
+module U8 = FStar.UInt8
+
+module U32 = FStar.UInt32
+
+module S = FStar.Seq
+
+
+
+(*
+A = 1 + D1 + D2 + ... + Dn (mod 65521)
+
+B = (1 + D1) + (1 + D1 + D2) + ... + (1 + D1 + D2 + ... + Dn) (mod 65521)
+  = n×D1 + (n−1)×D2 + (n−2)×D3 + ... + Dn + n (mod 65521)
+
+Adler32(D) = B × 65536 + A
+*)
+
+noextract
+let rec sum_plus_one (data: S.seq U8.t) : Tot nat (decreases (S.length data)) =
+  match S.length data with
+  | 0 -> 1
+  | _ -> (U8.v (S.head data)) + sum_plus_one (S.tail data)
+
+noextract
+let rec weighted_sum_plus_len (data: S.seq U8.t) : Tot nat (decreases (S.length data)) =
+  match S.length data with
+  | 0 -> 0
+  | _ -> 1 + ((S.length data) * (U8.v (S.head data))) + weighted_sum_plus_len (S.tail data)
+
+noextract
+let adler32 (data: S.seq U8.t) : Tot nat =
+  let a:nat = sum_plus_one (data) % 65521 in
+  let b:nat = weighted_sum_plus_len (data) % 65521 in
+  (b * (pow2 16)) + a
+
+#push-options "--max_fuel 20 --z3rlimit 20"
+
+noextract
+let test1_spec_adler32 () : unit =
+  let test_data:S.seq U8.t =
+    S.seq_of_list [U8.uint_to_t 4; U8.uint_to_t 1; U8.uint_to_t 6; U8.uint_to_t 3; U8.uint_to_t 10]
+  in
+  assert (weighted_sum_plus_len test_data == 63);
+  assert (sum_plus_one test_data == 25);
+  assert (adler32 test_data == 4128793); // 4128793 = 63 * (2^16) + 25
+  ()
+
+#pop-options
+
+noextract
+let test2_spec_adler32 () : unit =
+  let test_data:S.seq U8.t = S.seq_of_list [] in
+  assert (weighted_sum_plus_len test_data == 0);
+  assert (sum_plus_one test_data == 1);
+  assert (adler32 test_data == 1); // 1 = 0 * (2^16) + 1
+  ()
+
+noextract
+let test3_spec_adler32 () : unit =
+  let test_data:S.seq U8.t = S.seq_of_list [U8.uint_to_t 1] in
+  assert (weighted_sum_plus_len test_data == 2);
+  assert (sum_plus_one test_data == 2);
+  assert (adler32 test_data == 131074); // 131074 = 2 * (2^16) + 2
+  ()
