Makefile
@@ -1,31 +1,71 @@
-# Directories
+# Directoris
 OBJ_DIR = obj
 BUILD_DIR = build
 
-# Name
 NAME = adler32
 
 # Files
-FST_FILE = code/Impl.Adler32.fst
+FST_FILES = code/Impl.Adler32.fst code/Spec.Adler32.fst
+TEST_FILE = code/c/test.c
 KRML_OUTPUT = $(OBJ_DIR)/$(NAME).krml
-C_OUTPUT = $(BUILD_DIR)/$(NAME).c
-H_OUTPUT = $(BUILD_DIR)/$(NAME).h
-EXE_OUTPUT = $(BUILD_DIR)/$(NAME)
+
+C_FILE = $(BUILD_DIR)/$(NAME).c
+H_FILE = $(BUILD_DIR)/$(NAME).h
+OBJECT = $(BUILD_DIR)/$(NAME).o
+ARCHIVE = $(BUILD_DIR)/lib$(NAME).a
 
 # Default target
-all: $(C_OUTPUT) $(H_OUTPUT)
+# Generate archive
+$(ARCHIVE): $(OBJECT)
+	ar rcs $(ARCHIVE) $(OBJECT)
+
+# Generate Object file .o
+$(OBJECT): $(C_FILE)
+	ccomp \
+	-Wall \
+	-Werror \
+	-std=c11 \
+	-c $(C_FILE) \
+	-o $(OBJECT) 
+
+# Generate C and H file from .krml
+$(C_FILE) $(H_FILE): $(KRML_OUTPUT)
+	krml \
+	-skip-compilation \
+	-skip-makefiles \
+	-minimal \
+	-bundle 'Impl.Adler32=Impl.Adler32,Spec.Adler32,FStar.*,LowStar.*[rename=$(NAME)]' \
+	-drop Prims,C_Loops \
+	-add-include '<stdint.h>' \
+	-tmpdir $(BUILD_DIR) \
+	-no-prefix Impl.Adler32 \
+	$(KRML_OUTPUT) 
 
 # Generate the .krml file from F* code
-$(KRML_OUTPUT): $(FST_FILE)
-	fstar.exe --cache_dir $(OBJ_DIR) --codegen krml --krmloutput $(KRML_OUTPUT) $(FST_FILE)
+$(KRML_OUTPUT): $(FST_FILES)
+	mkdir --parent $(OBJ_DIR)
+	install -m 664 $(KRML_HOME)/krmllib/obj/* $(OBJ_DIR)
+	fstar.exe \
+	--codegen krml \
+	--krmloutput $(KRML_OUTPUT) \
+	--include $(FSTAR_HOME) \
+	--include $(KRML_HOME)/krmllib \
+	--cache_dir $(OBJ_DIR) \
+	--cache_checked_modules \
+	--already_cached 'Prims FStar LowStar C TestLib' \
+	$(FST_FILES)
 
-# Generate C and H files from .krml
-$(C_OUTPUT) $(H_OUTPUT): $(KRML_OUTPUT)
-	krml -tmpdir $(BUILD_DIR) -no-prefix $(basename $(notdir $(FST_FILE))) $(KRML_OUTPUT) -o $(EXE_OUTPUT)
+test: $(ARCHIVE) $(TEST_FILE) $(H_FILE)
+	@gcc $(TEST_FILE) -I$(BUILD_DIR) -L$(BUILD_DIR) -l$(NAME) -z noexecstack -o $(BUILD_DIR)/test
+	@$(BUILD_DIR)/test
+	@rm $(BUILD_DIR)/test
 
 # Clean up generated files
 clean:
 	rm -rf $(OBJ_DIR) $(BUILD_DIR)
+
+run:
+	@$(EXE_OUTPUT)	
 
 # Phony targets
 .PHONY: all clean
